(WIP) typos and experimental shit

WILLIS.dfy
@@ -3,7 +3,7 @@ include "Ownership-Parallel.dfy"
 include "Context.dfy"
 
 
-lemma All_Fucked_Up(obelow : Owner, oabove : Owner, cbelow : Owner, cabove : Owner, m : Klon)
+lemma {:verify false} All_Fucked_Up (obelow : Owner, oabove : Owner, cbelow : Owner, cabove : Owner, m : Klon)
   requires AllReady(obelow)
   requires AllReady(oabove)
   requires AllReady(cbelow)
@@ -16,5 +16,146 @@ lemma All_Fucked_Up(obelow : Owner, oabove : Owner, cbelow : Owner, cabove : Own
   requires cbelow == mapThruKlon(obelow, m)
   requires cabove == mapThruKlon(oabove, m)
 
-   ensures flatten(cbelow) >= flatten(cabove)
+//   ensures flatten(cbelow) >= flatten(cabove)
+{
+    var oaOF := allOutsideFlatten(obelow,m.o) - m.o.AMFO;
+    var caOF := allOutsideFlatten(cbelow,m.c) - m.c.AMFO;
+
+// assert oaOF == caOF; //shouldnt work!  //BUIT IT DOESS!!!!!!Q!
+
+    var oSBF := allStrictlyBelowFlatten(obelow,m.o);
+    var cSBF := allStrictlyBelowFlatten(cbelow,m.c);
+
+// assert cSBF == mapThruKlon(oSBF, m);
+
+
+}
+
+
+
+function allOutsideFlatten(ownrs : OWNR, pivot : Object) : (rv : Owner)
+ //or allFlatOutside or allOutsideFlat?    all => returns set;
+//flattens ownrs, returns all those that are outside/above the pivot
+  requires AllReady(flatten(ownrs))
+  requires pivot.Ready()
+  ensures AllReady(rv)
+{ set x <- flatten(ownrs) | outside(x,pivot) } // not(strictlyInside(x, pivot)) }
+
+
+function allStrictlyBelowFlatten(ownrs : OWNR, pivot : Object) : (rv : Owner)
+//flattens ownrs, returns all those that are strictlyInside/beloiw the pivot - or allStricltInsideFlat
+  requires AllReady(flatten(ownrs))
+  requires pivot.Ready()
+  ensures AllReady(rv)
+{ set x <- flatten(ownrs) | strictlyInside(x,pivot) } // not(strictlyInside(x, pivot)) }
+
+
+function allStrictlyBelowFlattenMap(ownrs : OWNR, m : Klon) : (rv : Owner)
+//maps owners thru klon, flattens ownrs, returns all those that are strictlyInside/beloiw the pivot
+     reads m.hns()
+  requires AllReady(flatten(ownrs))
+  requires klonReady(m)
+  requires klonCalid(m)
+  requires ownrs <= m.m.Keys
+
+   ensures AllReady(rv)
+   ensures forall r <- rv    :: strictlyInside(r, m.c)
+   ensures forall o <- ownrs :: klonLine(o, m.m[o], m)
+  // ensures rv <= m.m.Values
+  // ensures forall b <- mapBackKlon(rv,m) :: strictlyInside(b, m.o)
+{ set x : Object <- flatten(mapThruKlon(ownrs, m)) | strictlyInside(x, m.c) }
+
+
+
+
+
+
+
+
+
+
+
+function allOwnersInsidePivot(o : Object, pivot : Object) : (rv : Owner)
+//flattens ownrs, returns all those that are inside the pivot -
+  requires o.Ready()
+  requires pivot.Ready()
+   ensures AllReady(rv)
+   ensures forall r <- rv :: recInside(r, pivot)
+   ensures forall oo <- o.AMFO :: recInside(oo,pivot) ==> oo in rv
+   ensures forall r <- rv :: inside(r, pivot)
+   ensures forall oo <- o.AMFO :: inside(oo,pivot) ==> oo in rv
+ {
+     set x <- o.AMFO | inside(x,pivot)
+ }
+
+
+function allOwnersRecInsidePivot(o : Object, pivot : Object) : (rv : Owner)
+//flattens ownrs, returns all those that are inside the pivot -
+  requires o.Ready()
+  requires pivot.Ready()
+   ensures AllReady(rv)
+   ensures forall r <- rv :: recInside(r, pivot)
+   ensures forall oo <- o.AMFO :: recInside(oo,pivot) ==> oo in rv
+   ensures forall r <- rv :: inside(r, pivot)
+   ensures forall oo <- o.AMFO :: inside(oo,pivot) ==> oo in rv
+ {
+     set x <- o.AMFO | recInside(x,pivot)
+ }
+
+
+function allOwnersMinusPivot(o : Object, pivot : Object) : (rv : Owner)
+//flattens ownrs, returns all those that are strictlyInside/beloiw the pivot - or allStricltInsideFlat
+  requires o.Ready()
+  requires pivot.Ready()
+  requires strictlyInside(o,pivot)
+   ensures AllReady(rv)
+//   ensures forall r <- rv :: inside(r, pivot)
+   ensures forall oo <- o.AMFO :: inside(oo,pivot) ==> oo in rv
+ {
+     o.AMFO - pivot.AMFX
+ }
+
+
+
+lemma INSIDE_MINUS_PIVOT(o : Object, pivot : Object)
+   requires o.Ready()
+   requires pivot.Ready()
+   requires strictlyInside(o,pivot)
+    ensures allOwnersMinusPivot(o,pivot) == allOwnersInsidePivot(o,pivot)
+    ensures allOwnersMinusPivot(o,pivot) == allOwnersRecInsidePivot(o,pivot)
+    ensures allOwnersInsidePivot(o,pivot) == allOwnersRecInsidePivot(o,pivot)
 {}
+
+
+
+
+
+
+
+
+
+
+
+
+
+
+function allOwnersStrictlyInsidePivot(o : Object, pivot : Object) : (rv : Owner)
+//flattens ownrs, returns all those that are strictlyInside/beloiw the pivot - or allStricltInsideFlat
+  requires o.Ready()
+  requires pivot.Ready()
+   ensures AllReady(rv)
+   ensures forall r <- rv :: strictlyInside(r, pivot)
+ {
+     set x <- o.AMFO | strictlyInside(x,pivot)
+ }
+
+function allOwnersStrictlyMinusPivot(o : Object, pivot : Object) : (rv : Owner)
+//flattens ownrs, returns all those that are strictlyInside/beloiw the pivot - or allStricltInsideFlat
+  requires o.Ready()
+  requires pivot.Ready()
+  requires strictlyInside(o,pivot)
+   ensures AllReady(rv)
+//   ensures forall r <- rv :: strictlyInside(r, pivot)
+ {
+     o.AMFO - pivot.AMFO
+ }
